wip: transpose8x8 and transpose16x16

lib/Lib.IntVector.Transpose.fst
@@ -35,9 +35,8 @@ let transpose4x4 #t vs =
 ///
 
 inline_for_extraction noextract
-val transpose8x8_uint32: #t:v_inttype{t == U32} -> vec_t8 t -> vec_t8 t
-let transpose8x8_uint32 #t vs =
-  let (v0,v1,v2,v3,v4,v5,v6,v7) = vs in
+val transpose8x8_uint32_0: #t:v_inttype{t == U32} -> vec_t8 t -> vec_t8 t
+let transpose8x8_uint32_0 #t (v0,v1,v2,v3,v4,v5,v6,v7) =
   let v0' = vec_interleave_low v0 v1 in
   let v1' = vec_interleave_high v0 v1 in
   let v2' = vec_interleave_low v2 v3 in
@@ -46,25 +45,48 @@ let transpose8x8_uint32 #t vs =
   let v5' = vec_interleave_high v4 v5 in
   let v6' = vec_interleave_low v6 v7 in
   let v7' = vec_interleave_high v6 v7 in
+  (v0',v1',v2',v3',v4',v5',v6',v7')
 
-  let v0'' = vec_interleave_low_n 2 v0' v2' in
-  let v1'' = vec_interleave_high_n 2 v0' v2' in
-  let v2'' = vec_interleave_low_n 2 v1' v3' in
-  let v3'' = vec_interleave_high_n 2 v1' v3' in
-  let v4'' = vec_interleave_low_n 2 v4' v6' in
-  let v5'' = vec_interleave_high_n 2 v4' v6' in
-  let v6'' = vec_interleave_low_n 2 v5' v7' in
-  let v7'' = vec_interleave_high_n 2 v5' v7' in
 
-  let v0''' = vec_interleave_low_n 4 v0'' v4'' in
-  let v1''' = vec_interleave_high_n 4 v0'' v4'' in
-  let v2''' = vec_interleave_low_n 4 v1'' v5'' in
-  let v3''' = vec_interleave_high_n 4 v1'' v5'' in
-  let v4''' = vec_interleave_low_n 4 v2'' v6'' in
-  let v5''' = vec_interleave_high_n 4 v2'' v6'' in
-  let v6''' = vec_interleave_low_n 4 v3'' v7'' in
-  let v7''' = vec_interleave_high_n 4 v3'' v7'' in
-  (v0''',v2''',v4''',v6''',v1''',v3''',v5''',v7''')
+inline_for_extraction noextract
+val transpose8x8_uint32_1: #t:v_inttype{t == U32} -> vec_t8 t -> vec_t8 t
+let transpose8x8_uint32_1 #t (v0,v1,v2,v3,v4,v5,v6,v7) =
+  let v0' = vec_interleave_low_n 2 v0 v2 in
+  let v2' = vec_interleave_high_n 2 v0 v2 in
+  let v1' = vec_interleave_low_n 2 v1 v3 in
+  let v3' = vec_interleave_high_n 2 v1 v3 in
+  let v4' = vec_interleave_low_n 2 v4 v6 in
+  let v6' = vec_interleave_high_n 2 v4 v6 in
+  let v5' = vec_interleave_low_n 2 v5 v7 in
+  let v7' = vec_interleave_high_n 2 v5 v7 in
+  (v0',v1',v2',v3',v4',v5',v6',v7')
+
+
+inline_for_extraction noextract
+val transpose8x8_uint32_2: #t:v_inttype{t == U32} -> vec_t8 t -> vec_t8 t
+let transpose8x8_uint32_2 #t (v0,v1,v2,v3,v4,v5,v6,v7) =
+  let v0' = vec_interleave_low_n 4 v0 v4 in
+  let v4' = vec_interleave_high_n 4 v0 v4 in
+  let v1' = vec_interleave_low_n 4 v1 v5 in
+  let v5' = vec_interleave_high_n 4 v1 v5 in
+  let v2' = vec_interleave_low_n 4 v2 v6 in
+  let v6' = vec_interleave_high_n 4 v2 v6 in
+  let v3' = vec_interleave_low_n 4 v3 v7 in
+  let v7' = vec_interleave_high_n 4 v3 v7 in
+  (v0',v1',v2',v3',v4',v5',v6',v7')
+
+
+inline_for_extraction noextract
+val transpose8x8_uint32: #t:v_inttype{t == U32} -> vec_t8 t -> vec_t8 t
+let transpose8x8_uint32 #t vs0 =
+  let (v0,v1,v2,v3,v4,v5,v6,v7) = vs0 in
+  [@inline_let]
+  let (v0',v1',v2',v3',v4',v5',v6',v7') = transpose8x8_uint32_0 #t (v0,v1,v2,v3,v4,v5,v6,v7) in
+  [@inline_let]
+  let (v0',v1',v2',v3',v4',v5',v6',v7') = transpose8x8_uint32_1 #t (v0',v1',v2',v3',v4',v5',v6',v7') in
+  [@inline_let]
+  let (v0',v1',v2',v3',v4',v5',v6',v7') = transpose8x8_uint32_2 #t (v0',v1',v2',v3',v4',v5',v6',v7') in
+  (v0',v2',v1',v3',v4',v6',v5',v7')
 
 let transpose8x8 #t vs =
   match t with
@@ -73,8 +95,8 @@ let transpose8x8 #t vs =
 
 
 inline_for_extraction noextract
-val transpose16x16_uint32: #t:v_inttype{t == U32} -> vs:(vec_t16 t & vec_t16 t) -> (vec_t16 t & vec_t16 t)
-let transpose16x16_uint32 #t vs =
+val transpose16x16_uint32_0: #t:v_inttype{t == U32} -> vs:(vec_t16 t & vec_t16 t) -> (vec_t16 t & vec_t16 t)
+let transpose16x16_uint32_0 #t vs =
   let ((v0,v1,v2,v3,v4,v5,v6,v7),(v8,v9,v10,v11,v12,v13,v14,v15)) = vs in
 
   let v0' = vec_interleave_low v0 v1 in
@@ -94,56 +116,103 @@ let transpose16x16_uint32 #t vs =
   let v14' = vec_interleave_low v14 v15 in
   let v15' = vec_interleave_high v14 v15 in
 
-  let v0'' = vec_interleave_low_n 2 v0' v2' in
-  let v2'' = vec_interleave_high_n 2 v0' v2' in
-  let v1'' = vec_interleave_low_n 2 v1' v3' in
-  let v3'' = vec_interleave_high_n 2 v1' v3' in
-  let v4'' = vec_interleave_low_n 2 v4' v6' in
-  let v6'' = vec_interleave_high_n 2 v4' v6' in
-  let v5'' = vec_interleave_low_n 2 v5' v7' in
-  let v7'' = vec_interleave_high_n 2 v5' v7' in
-  let v8'' = vec_interleave_low_n 2 v8' v10' in
-  let v10'' = vec_interleave_high_n 2 v8' v10' in
-  let v9'' = vec_interleave_low_n 2 v9' v11' in
-  let v11'' = vec_interleave_high_n 2 v9' v11' in
-  let v12'' = vec_interleave_low_n 2 v12' v14' in
-  let v14'' = vec_interleave_high_n 2 v12' v14' in
-  let v13'' = vec_interleave_low_n 2 v13' v15' in
-  let v15'' = vec_interleave_high_n 2 v13' v15' in
+  ((v0',v1',v2',v3',v4',v5',v6',v7'),(v8',v9',v10',v11',v12',v13',v14',v15'))
 
-  let v0' = vec_interleave_low_n 4 v0'' v4'' in
-  let v4' = vec_interleave_high_n 4 v0'' v4'' in
-  let v1' = vec_interleave_low_n 4 v1'' v5'' in
-  let v5' = vec_interleave_high_n 4 v1'' v5'' in
-  let v2' = vec_interleave_low_n 4 v2'' v6'' in
-  let v6' = vec_interleave_high_n 4 v2'' v6'' in
-  let v3' = vec_interleave_low_n 4 v3'' v7'' in
-  let v7' = vec_interleave_high_n 4 v3'' v7'' in
-  let v8' = vec_interleave_low_n 4 v8'' v12'' in
-  let v12' = vec_interleave_high_n 4 v8'' v12'' in
-  let v9' = vec_interleave_low_n 4 v9'' v13'' in
-  let v13' = vec_interleave_high_n 4 v9'' v13'' in
-  let v10' = vec_interleave_low_n 4 v10'' v14'' in
-  let v14' = vec_interleave_high_n 4 v10'' v14'' in
 
-  let v0 = vec_interleave_low_n 8 v0' v8' in
-  let v8 = vec_interleave_high_n 8 v0' v8' in
-  let v1 = vec_interleave_low_n 8 v1' v9' in
-  let v9 = vec_interleave_high_n 8 v1' v9' in
-  let v2 = vec_interleave_low_n 8 v2' v10' in
-  let v10 = vec_interleave_high_n 8 v2' v10' in
-  let v3 = vec_interleave_low_n 8 v3' v11' in
-  let v11 = vec_interleave_high_n 8 v3' v11' in
-  let v4 = vec_interleave_low_n 8 v4' v12' in
-  let v12 = vec_interleave_high_n 8 v4' v12' in
-  let v5 = vec_interleave_low_n 8 v5' v13' in
-  let v13 = vec_interleave_high_n 8 v5' v13' in
-  let v6 = vec_interleave_low_n 8 v6' v14' in
-  let v14 = vec_interleave_high_n 8 v6' v14' in
-  let v7 = vec_interleave_low_n 8 v7' v15' in
-  let v15 = vec_interleave_high_n 8 v7' v15' in
+inline_for_extraction noextract
+val transpose16x16_uint32_1: #t:v_inttype{t == U32} -> vs:(vec_t16 t & vec_t16 t) -> (vec_t16 t & vec_t16 t)
+let transpose16x16_uint32_1 #t vs =
+  let ((v0,v1,v2,v3,v4,v5,v6,v7),(v8,v9,v10,v11,v12,v13,v14,v15)) = vs in
 
-  (v0,v2,v1,v3,v4,v6,v5,v7), (v8,v10,v9,v11,v12,v14,v13,v15)
+  let v0' = vec_interleave_low_n 2 v0 v2 in
+  let v2' = vec_interleave_high_n 2 v0 v2 in
+  let v1' = vec_interleave_low_n 2 v1 v3 in
+  let v3' = vec_interleave_high_n 2 v1 v3 in
+  let v4' = vec_interleave_low_n 2 v4 v6 in
+  let v6' = vec_interleave_high_n 2 v4 v6 in
+  let v5' = vec_interleave_low_n 2 v5 v7 in
+  let v7' = vec_interleave_high_n 2 v5 v7 in
+  let v8' = vec_interleave_low_n 2 v8 v10 in
+  let v10' = vec_interleave_high_n 2 v8 v10 in
+  let v9' = vec_interleave_low_n 2 v9 v11 in
+  let v11' = vec_interleave_high_n 2 v9 v11 in
+  let v12' = vec_interleave_low_n 2 v12 v14 in
+  let v14' = vec_interleave_high_n 2 v12 v14 in
+  let v13' = vec_interleave_low_n 2 v13 v15 in
+  let v15' = vec_interleave_high_n 2 v13 v15 in
+
+  ((v0',v1',v2',v3',v4',v5',v6',v7'),(v8',v9',v10',v11',v12',v13',v14',v15'))
+
+
+inline_for_extraction noextract
+val transpose16x16_uint32_2: #t:v_inttype{t == U32} -> vs:(vec_t16 t & vec_t16 t) -> (vec_t16 t & vec_t16 t)
+let transpose16x16_uint32_2 #t vs =
+  let ((v0,v1,v2,v3,v4,v5,v6,v7),(v8,v9,v10,v11,v12,v13,v14,v15)) = vs in
+
+  let v0' = vec_interleave_low_n 4 v0 v4 in
+  let v4' = vec_interleave_high_n 4 v0 v4 in
+  let v1' = vec_interleave_low_n 4 v1 v5 in
+  let v5' = vec_interleave_high_n 4 v1 v5 in
+  let v2' = vec_interleave_low_n 4 v2 v6 in
+  let v6' = vec_interleave_high_n 4 v2 v6 in
+  let v3' = vec_interleave_low_n 4 v3 v7 in
+  let v7' = vec_interleave_high_n 4 v3 v7 in
+  let v8' = vec_interleave_low_n 4 v8 v12 in
+  let v12' = vec_interleave_high_n 4 v8 v12 in
+  let v9' = vec_interleave_low_n 4 v9 v13 in
+  let v13' = vec_interleave_high_n 4 v9 v13 in
+  let v10' = vec_interleave_low_n 4 v10 v14 in
+  let v14' = vec_interleave_high_n 4 v10 v14 in
+  let v11' = vec_interleave_low_n 4 v11 v15 in
+  let v15' = vec_interleave_high_n 4 v11 v15 in
+
+  ((v0',v1',v2',v3',v4',v5',v6',v7'),(v8',v9',v10',v11',v12',v13',v14',v15'))
+
+
+inline_for_extraction noextract
+val transpose16x16_uint32_3: #t:v_inttype{t == U32} -> vs:(vec_t16 t & vec_t16 t) -> (vec_t16 t & vec_t16 t)
+let transpose16x16_uint32_3 #t vs =
+  let ((v0,v1,v2,v3,v4,v5,v6,v7),(v8,v9,v10,v11,v12,v13,v14,v15)) = vs in
+
+  let v0' = vec_interleave_low_n 8 v0 v8 in
+  let v8' = vec_interleave_high_n 8 v0 v8 in
+  let v1' = vec_interleave_low_n 8 v1 v9 in
+  let v9' = vec_interleave_high_n 8 v1 v9 in
+  let v2' = vec_interleave_low_n 8 v2 v10 in
+  let v10' = vec_interleave_high_n 8 v2 v10 in
+  let v3' = vec_interleave_low_n 8 v3 v11 in
+  let v11' = vec_interleave_high_n 8 v3 v11 in
+  let v4' = vec_interleave_low_n 8 v4 v12 in
+  let v12' = vec_interleave_high_n 8 v4 v12 in
+  let v5' = vec_interleave_low_n 8 v5 v13 in
+  let v13' = vec_interleave_high_n 8 v5 v13 in
+  let v6' = vec_interleave_low_n 8 v6 v14 in
+  let v14' = vec_interleave_high_n 8 v6 v14 in
+  let v7' = vec_interleave_low_n 8 v7 v15 in
+  let v15' = vec_interleave_high_n 8 v7 v15 in
+
+  ((v0',v1',v2',v3',v4',v5',v6',v7'),(v8',v9',v10',v11',v12',v13',v14',v15'))
+
+
+inline_for_extraction noextract
+val transpose16x16_uint32: #t:v_inttype{t == U32} -> vs:(vec_t16 t & vec_t16 t) -> (vec_t16 t & vec_t16 t)
+let transpose16x16_uint32 #t vs =
+  let ((v0,v1,v2,v3,v4,v5,v6,v7),(v8,v9,v10,v11,v12,v13,v14,v15)) = vs in
+
+  [@inline_let]
+  let ((v0',v1',v2',v3',v4',v5',v6',v7'),(v8',v9',v10',v11',v12',v13',v14',v15')) =
+    transpose16x16_uint32_0 ((v0,v1,v2,v3,v4,v5,v6,v7),(v8,v9,v10,v11,v12,v13,v14,v15)) in
+  [@inline_let]
+  let ((v0',v1',v2',v3',v4',v5',v6',v7'),(v8',v9',v10',v11',v12',v13',v14',v15')) =
+    transpose16x16_uint32_1 ((v0',v1',v2',v3',v4',v5',v6',v7'),(v8',v9',v10',v11',v12',v13',v14',v15')) in
+  [@inline_let]
+  let ((v0',v1',v2',v3',v4',v5',v6',v7'),(v8',v9',v10',v11',v12',v13',v14',v15')) =
+    transpose16x16_uint32_2 ((v0',v1',v2',v3',v4',v5',v6',v7'),(v8',v9',v10',v11',v12',v13',v14',v15')) in
+  [@inline_let]
+  let ((v0',v1',v2',v3',v4',v5',v6',v7'),(v8',v9',v10',v11',v12',v13',v14',v15')) =
+    transpose16x16_uint32_3 ((v0',v1',v2',v3',v4',v5',v6',v7'),(v8',v9',v10',v11',v12',v13',v14',v15')) in
+
+  ((v0',v2',v1',v3',v4',v6',v5',v7'),(v8',v10',v9',v11',v12',v14',v13',v15'))
 
 
 let transpose16x16 #t vs =
@@ -199,7 +268,13 @@ let transpose4x4_lseq_is_transposewxw_uint32 vs0 =
   Loops.eq_repeati0 n (transposewxw_uint32_f #4 n) vs0
 
 
-#push-options "--fuel 1"
+inline_for_extraction noextract
+let f_lseq8 (#t:v_inttype) (vs:lseq (vec_t t 8) 8) (f:vec_t8 t -> vec_t8 t) : lseq (vec_t t 8) 8 =
+  let (v0,v1,v2,v3,v4,v5,v6,v7) = (vs.[0],vs.[1],vs.[2],vs.[3],vs.[4],vs.[5],vs.[6],vs.[7]) in
+  let (r0,r1,r2,r3,r4,r5,r6,r7) = f (v0,v1,v2,v3,v4,v5,v6,v7) in
+  create8 r0 r1 r2 r3 r4 r5 r6 r7
+
+
 val transpose8x8_lseq_is_transposewxw_uint32: vs:lseq (vec_t U32 8) 8 ->
   Lemma
    (let r = transposewxw_uint32_lseq 3 vs in
@@ -211,13 +286,29 @@ let transpose8x8_lseq_is_transposewxw_uint32 vs0 =
   Loops.unfold_repeati n (transposewxw_uint32_f #8 n) vs0 1;
   Loops.unfold_repeati n (transposewxw_uint32_f #8 n) vs0 0;
   Loops.eq_repeati0 n (transposewxw_uint32_f #8 n) vs0;
-  //let r = transposewxw_uint32_lseq 3 vs0 in
-  //eq_intro (create8 r.[0] r.[2] r.[1] r.[3] r.[4] r.[6] r.[5] r.[7]) (transpose8x8_lseq #U32 vs0)
-  admit()
-#pop-options
+  let r = transposewxw_uint32_lseq 3 vs0 in
+  let res = create8 r.[0] r.[2] r.[1] r.[3] r.[4] r.[6] r.[5] r.[7] in
+
+  let res0 = transposewxw_uint32_f n 0 vs0 in
+  eq_intro res0 (f_lseq8 vs0 transpose8x8_uint32_0);
+  let res1 = transposewxw_uint32_f n 1 res0 in
+  eq_intro res1 (f_lseq8 res0 transpose8x8_uint32_1);
+  let res2 = transposewxw_uint32_f n 2 res1 in
+  eq_intro res2 (f_lseq8 res1 transpose8x8_uint32_2);
+  eq_intro res (f_lseq8 vs0 transpose8x8)
 
 
-#push-options "--fuel 1"
+inline_for_extraction noextract
+let f_lseq16 (#t:v_inttype) (vs:lseq (vec_t t 16) 16)
+  (f:(vec_t16 t & vec_t16 t -> vec_t16 t & vec_t16 t)) : lseq (vec_t t 16) 16
+ =
+  let (v0,v1,v2,v3,v4,v5,v6,v7) = (vs.[0],vs.[1],vs.[2],vs.[3],vs.[4],vs.[5],vs.[6],vs.[7]) in
+  let (v8,v9,v10,v11,v12,v13,v14,v15) = (vs.[8],vs.[9],vs.[10],vs.[11],vs.[12],vs.[13],vs.[14],vs.[15]) in
+  let ((r0,r1,r2,r3,r4,r5,r6,r7),(r8,r9,r10,r11,r12,r13,r14,r15)) =
+    f ((v0,v1,v2,v3,v4,v5,v6,v7), (v8,v9,v10,v11,v12,v13,v14,v15)) in
+  create16 r0 r1 r2 r3 r4 r5 r6 r7 r8 r9 r10 r11 r12 r13 r14 r15
+
+
 val transpose16x16_lseq_is_transposewxw_uint32: vs:lseq (vec_t U32 16) 16 ->
   Lemma
    (let r = transposewxw_uint32_lseq 4 vs in
@@ -232,11 +323,18 @@ let transpose16x16_lseq_is_transposewxw_uint32 vs0 =
   Loops.unfold_repeati n (transposewxw_uint32_f #16 n) vs0 0;
   Loops.eq_repeati0 n (transposewxw_uint32_f #16 n) vs0;
   let r = transposewxw_uint32_lseq n vs0 in
-  let res_wxw = create16 r.[0] r.[2] r.[1] r.[3] r.[4] r.[6] r.[5] r.[7] r.[8] r.[10] r.[9] r.[11] r.[12] r.[14] r.[13] r.[15] in
-  let res = transpose16x16_lseq #U32 vs0 in
-  //eq_intro res_wxw res;
-  admit()
-#pop-options
+
+  let res0 = transposewxw_uint32_f n 0 vs0 in
+  eq_intro res0 (f_lseq16 vs0 transpose16x16_uint32_0);
+  let res1 = transposewxw_uint32_f n 1 res0 in
+  eq_intro res1 (f_lseq16 res0 transpose16x16_uint32_1);
+  let res2 = transposewxw_uint32_f n 2 res1 in
+  eq_intro res2 (f_lseq16 res1 transpose16x16_uint32_2);
+  let res3 = transposewxw_uint32_f n 3 res2 in
+  eq_intro res3 (f_lseq16 res2 transpose16x16_uint32_3);
+  let res = create16 r.[0] r.[2] r.[1] r.[3] r.[4] r.[6] r.[5] r.[7] r.[8] r.[10] r.[9] r.[11] r.[12] r.[14] r.[13] r.[15] in
+  eq_intro res (f_lseq16 vs0 transpose16x16_uint32)
+
 
 val transpose4x4_lemma_ij: vs:lseq (vec_t U32 4) 4 -> i:nat{i < 4} -> j:nat{j < 4} ->
   Lemma ((vec_v (transpose4x4_lseq #U32 vs).[i]).[j] == (vec_v vs.[j]).[i])
